Corpus/coverage/exec/multipkg/private-method-dispatch/red/inner/inner.go
@@ -1,0 +1,33 @@
+package inner
+
+type A int
+
+func (a A) m() int { return 100 + int(a) }
+func (a A) É() int { return 300 + int(a) }
+func (a A) é() int { return 400 + int(a) }
+func (a A) 𐐀() int { return 500 + int(a) }
+
+type I interface{ m() int }
+type Unicode interface {
+	é() int
+	É() int
+	𐐀() int
+}
+
+func Read(x I) int                          { return x.m() }
+func Value(x I) int                         { f := x.m; return f() }
+func Expr(x I) int                          { return I.m(x) }
+func Is(x any) bool                         { _, ok := x.(I); return ok }
+func UnicodeRead(x Unicode) (int, int, int) { return x.é(), x.É(), x.𐐀() }
+func ConcreteValue(a A) int                 { f := a.m; return f() }
+func ConcreteExpr(a A) int                  { return A.m(a) }
+
+type P int
+
+func (p *P) m() int { return 600 + int(*p) }
+
+type G[T ~int] struct{ V T }
+
+func (g G[T]) m() int                              { f := func() int { return 700 + int(g.V) }; return f() }
+func GenericRead[T interface{ m() int }](x T) int  { return x.m() }
+func GenericValue[T interface{ m() int }](x T) int { f := x.m; return f() }
